A first attempt at an adder-tree

cava-examples/AdderTree.v
@@ -24,6 +24,8 @@ From Coq Require Import Bool.Bool.
 From Coq Require Import Ascii String.
 From Coq Require Import Lists.List.
 From Coq Require Import NArith.
+From Coq Require Import Vector.
+From Coq Require Import Bool.Bvector.
 Import ListNotations.
 
 Require Import ExtLib.Structures.Monads.
@@ -35,8 +37,12 @@ Require Import Cava.Combinators.
 Require Import Cava.Netlist.
 Require Import Cava.BitArithmetic.
 
+Require Import Nat Arith Lia.
+
 Local Open Scope list_scope.
 Local Open Scope monad_scope.
+
+Set Implicit Arguments.
 
 
 Definition adder_3in {m bit} `{Cava m bit} {aL bL cL : nat}
@@ -58,4 +64,136 @@ Definition adder8_3inTop : state CavaState (Vector.t N 10) :=
   outputVectorTo0 10 sum "sum".
 
 Definition adder8_3inNetlist := makeNetlist adder8_3inTop.
-  
+
+Lemma add3_behaviour : forall aL bL cL (av : Bvector aL) (bv : Bvector bL) (cv : Bvector cL),
+                       let a := bitvec_to_nat av in
+                       let b := bitvec_to_nat bv in
+                       let c := bitvec_to_nat cv in
+                       bitvec_to_nat (combinational (adder_3in av bv cv)) = a + b + c.
+Proof.
+  intros. unfold combinational. unfold adder_3in. simpl. rewrite bvnat. rewrite bvnat.
+  reflexivity.
+Qed.
+
+Lemma max_x_x : forall x, max x x = x.
+Proof.
+ intro x. induction x. simpl. auto. simpl. rewrite IHx. reflexivity.
+Defined.
+
+Definition simplify_max {a n} (x : Vector.t a (max n n + 1)) : Vector.t a (n + 1).
+  rewrite max_x_x in x.
+  auto.
+Defined.
+
+Definition adderFixed {m bit} `{Cava m bit} {l : nat}
+                      (a : (Vector.t bit l))
+                      (b : (Vector.t bit l))
+                      : m (Vector.t bit (l + 1)) :=
+  a_plus_b <- unsignedAdd a b ;;
+  ret (simplify_max a_plus_b).
+
+Definition adder_fixed_top : state CavaState (Vector.t N 9) :=
+  setModuleName "adder_fixed" ;;
+  a <- inputVectorTo0 8 "a" ;;
+  b <- inputVectorTo0 8 "b" ;;
+  sum <- adderFixed a b ;;
+  outputVectorTo0 9 sum "sum".
+
+Definition adder_fixedNetlist := makeNetlist adder_fixed_top.
+
+Definition v0 := nat_to_bitvec 8  4.
+Definition v1 := nat_to_bitvec 8 17.
+Definition v2 := nat_to_bitvec 8  6.
+Definition v3 := nat_to_bitvec 8  3.
+
+Example check_fixed: bitvec_to_nat (combinational (adderFixed v0 v1)) = 21.
+Proof. reflexivity. Qed.
+
+(* TODO(satnam): track down a library that must contain this lemma. *)
+Lemma add_1_r : forall n, S n = n + 1.
+Proof.
+  intros. induction n.
+  - simpl. reflexivity.
+  - simpl. rewrite IHn. reflexivity.
+Defined.
+
+(* To create an adder with no bit-growth at the output we need to be able
+   to discard the top bit, producing a add-modulo unsigned adder.
+*)
+Definition discardTopBit {a n} (v : Vector.t a (n+1)) : Vector.t a n.
+  apply shiftout.
+  rewrite add_1_r.
+  auto.
+Defined.
+
+Definition adderNoGrowth {m bit} `{C : Cava m bit} {l : nat}
+                         (a : (Vector.t bit l))
+                         (b : (Vector.t bit l))
+                         : m (Vector.t bit l) :=
+  a_plus_b <- adderFixed a b ;;
+  ret (discardTopBit a_plus_b).
+
+Definition to_n_plus_n {a n} (v : Vector.t a (2*n)) : Vector.t a (n + n).
+Proof.
+  intros. simpl in v. rewrite <- plus_n_O in v. apply v.
+Defined.
+
+Definition halve' {n a} (v : Vector.t a (n+n)) : Vector.t a n * Vector.t a n :=
+  splitat n v.
+
+Definition v0_3 : Vector.t (Bvector 8) (2+2) := [v0; v1; v2; v3]%vector.
+Compute halve' v0_3.
+
+Definition halve {n a} (v : Vector.t a (2*n)) : Vector.t a n * Vector.t a n :=
+  halve' (to_n_plus_n v).
+
+Fixpoint adderTree {m bit} `{Cava m bit} (n s : nat) (v : Vector.t (Vector.t bit s) (2^(n+1))) : m (Vector.t bit s) :=
+  match n, v with
+  | O, v2 => adderNoGrowth (hd v2) (hd (tl v2))
+  | S n', vR => let '(vL, vH) := halve vR in
+                aS <- adderTree n' vL ;;
+                bS <- adderTree n' vH ;;
+                sum <- adderNoGrowth aS bS ;;
+                ret sum
+  end.
+ 
+(* An adder tree with 2 inputs each of 8 bits in size. *)
+
+Definition adderTree2_8 {m bit} `{Cava m bit} (v : Vector.t (Vector.t bit 8) 2) : m (Vector.t bit 8)
+  := adderTree 0 v.
+
+Definition v2_8 : Vector.t (Bvector 8) 2 := [v0; v1]%vector.
+Definition v0_plus_v1 : Bvector 8 := combinational (adderTree2_8 v2_8).
+Compute v0_plus_v1.
+
+Example v0_plus_v1_ex : bitvec_to_nat v0_plus_v1 = 21.
+Proof. reflexivity. Qed.
+
+(* An adder tree with 4 inputs each of 8 bits in size. *)
+
+Definition adderTree4_8 {m bit} `{Cava m bit} (v : Vector.t (Vector.t bit 8) 4) : m (Vector.t bit 8)
+  := adderTree 1 v.
+
+Definition adder_tree_4_8_top : state CavaState (Vector.t N 8) :=
+  setModuleName "adder_tree_4_8" ;;
+  a <- inputVectorTo0 8 "a" ;;
+  b <- inputVectorTo0 8 "b" ;;
+  c <- inputVectorTo0 8 "c" ;;
+  d <- inputVectorTo0 8 "d" ;;
+  sum <- adderTree4_8 [a; b; c; d]%vector ;;
+  outputVectorTo0 8 sum "sum".
+
+Definition adder_tree_4_8Netlist := makeNetlist adder_tree_4_8_top.
+
+Definition v4_8 : Vector.t (Bvector 8) (2^(1+1)) := [v0; v1; v2; v3]%vector.
+
+Definition adderTree4_8_sim : ident (Vector.t bool 8) := adderTree4_8 v4_8.
+
+(* This computation causes Coq to loop.
+Compute (combinational adderTree4_8_sim).
+*)
+
+(* This computation causes Coq to loop.
+Compute (combinational adderTree4_8_sim).
+*)
+
